theories/program_logic/adequacy.v
@@ -1,37 +1,10 @@
 From stdpp Require Import namespaces.
 From iris.program_logic Require Export weakestpre.
 From iris.algebra Require Import gmap auth agree gset coPset.
-From iris.base_logic.lib Require Import wsat.
+From iris.base_logic.lib Require Export wsat.
 From iris.proofmode Require Import tactics.
 Set Default Proof Using "Type".
 Import uPred.
-
-(* Global functor setup *)
-Definition invΣ : gFunctors :=
-  #[GFunctor (authRF (gmapURF positive (agreeRF (laterCF idCF))));
-    GFunctor coPset_disjUR;
-    GFunctor (gset_disjUR positive)].
-
-Class invPreG (Σ : gFunctors) : Set := WsatPreG {
-  inv_inPreG :> inG Σ (authR (gmapUR positive (agreeR (laterC (iPreProp Σ)))));
-  enabled_inPreG :> inG Σ coPset_disjR;
-  disabled_inPreG :> inG Σ (gset_disjR positive);
-}.
-
-Instance subG_invΣ {Σ} : subG invΣ Σ → invPreG Σ.
-Proof. solve_inG. Qed.
-
-(* Allocation *)
-Lemma wsat_alloc `{invPreG Σ} : (|==> ∃ _ : invG Σ, wsat ∗ ownE ⊤)%I.
-Proof.
-  iIntros.
-  iMod (own_alloc (● (∅ : gmap _ _))) as (γI) "HI"; first done.
-  iMod (own_alloc (CoPset ⊤)) as (γE) "HE"; first done.
-  iMod (own_alloc (GSet ∅)) as (γD) "HD"; first done.
-  iModIntro; iExists (WsatG _ _ _ _ γI γE γD).
-  rewrite /wsat /ownE -lock; iFrame.
-  iExists ∅. rewrite fmap_empty big_opM_empty. by iFrame.
-Qed.
 
 (* Program logic adequacy *)
 Record adequate {Λ} (s : stuckness) (e1 : expr Λ) (σ1 : state Λ)
@@ -66,28 +39,25 @@ Implicit Types P Q : iProp Σ.
 Implicit Types Φ : val Λ → iProp Σ.
 Implicit Types Φs : list (val Λ → iProp Σ).
 
-Notation world' E σ κs := (wsat ∗ ownE E ∗ state_interp σ κs)%I (only parsing).
-Notation world σ κs := (world' ⊤ σ κs) (only parsing).
-
 Notation wptp s t := ([∗ list] ef ∈ t, WP ef @ s; ⊤ {{ _, True }})%I.
 
 Lemma wp_step s E e1 σ1 κ κs e2 σ2 efs Φ :
   prim_step e1 σ1 κ e2 σ2 efs →
-  world' E σ1 (κ ++ κs) ∗ WP e1 @ s; E {{ Φ }}
-  ==∗  ▷ |==> ◇ (world' E σ2 κs ∗ WP e2 @ s; E {{ Φ }} ∗ wptp s efs).
+  state_interp σ1 (κ ++ κs) ∗ WP e1 @ s; E {{ Φ }}
+  ={E, ∅}▷=∗ (state_interp σ2 κs ∗ WP e2 @ s; E {{ Φ }} ∗ wptp s efs).
 Proof.
-  rewrite {1}wp_unfold /wp_pre. iIntros (?) "[(Hw & HE & Hσ) H]".
-  rewrite (val_stuck e1 σ1 κ e2 σ2 efs) // uPred_fupd_eq.
-  iMod ("H" $! σ1 with "Hσ [Hw HE]") as ">(Hw & HE & _ & H)"; first by iFrame.
-  iMod ("H" $! e2 σ2 efs with "[//] [$Hw $HE]") as ">(Hw & HE & H)".
-  iIntros "!> !>". by iMod ("H" with "[$Hw $HE]") as ">($ & $ & $)".
+  rewrite {1}wp_unfold /wp_pre. iIntros (?) "[Hσ H]".
+  rewrite (val_stuck e1 σ1 κ e2 σ2 efs) //.
+  iMod ("H" $! σ1 with "Hσ") as "(_ & H)".
+  iMod ("H" $! e2 σ2 efs with "[//]") as "H".
+  by iIntros "!> !>".
 Qed.
 
 Lemma wptp_step s e1 t1 t2 κ κs σ1 σ2 Φ :
   step (e1 :: t1,σ1) κ (t2, σ2) →
-  world σ1 (κ ++ κs) ∗ WP e1 @ s; ⊤ {{ Φ }} ∗ wptp s t1
+  state_interp σ1 (κ ++ κs) ∗ WP e1 @ s; ⊤ {{ Φ }} ∗ wptp s t1
   ==∗ ∃ e2 t2',
-    ⌜t2 = e2 :: t2'⌝ ∗ ▷ |==> ◇ (world σ2 κs ∗ WP e2 @ s; ⊤ {{ Φ }} ∗ wptp s t2').
+    ⌜t2 = e2 :: t2'⌝ ∗ |={⊤, ∅}▷=> (state_interp σ2 κs ∗ WP e2 @ s; ⊤ {{ Φ }} ∗ wptp s t2').
 Proof.
   iIntros (Hstep) "(HW & He & Ht)".
   destruct Hstep as [e1' σ1' e2' σ2' efs [|? t1'] t2' ?? Hstep]; simplify_eq/=.
@@ -100,77 +70,70 @@ Qed.
 
 Lemma wptp_steps s n e1 t1 κs κs' t2 σ1 σ2 Φ :
   nsteps n (e1 :: t1, σ1) κs (t2, σ2) →
-  world σ1 (κs ++ κs') ∗ WP e1 @ s; ⊤ {{ Φ }} ∗ wptp s t1 ⊢
-  Nat.iter (S n) (λ P, |==> ▷ P) (∃ e2 t2',
-    ⌜t2 = e2 :: t2'⌝ ∗ world σ2 κs' ∗ WP e2 @ s; ⊤ {{ Φ }} ∗ wptp s t2').
+  state_interp σ1 (κs ++ κs') ∗ WP e1 @ s; ⊤ {{ Φ }} ∗ wptp s t1 ⊢
+  |={⊤, ∅}▷=>^n (∃ e2 t2',
+    ⌜t2 = e2 :: t2'⌝ ∗ state_interp σ2 κs' ∗ WP e2 @ s; ⊤ {{ Φ }} ∗ wptp s t2').
 Proof.
   revert e1 t1 κs κs' t2 σ1 σ2; simpl; induction n as [|n IH]=> e1 t1 κs κs' t2 σ1 σ2 /=.
-  { inversion_clear 1; iIntros "?"; eauto 10. }
+  { inversion_clear 1; iIntros "(?&?&?)"; iExists e1, t1; iFrame; eauto 10. }
   iIntros (Hsteps) "H". inversion_clear Hsteps as [|?? [t1' σ1']].
   rewrite <- app_assoc.
-  iMod (wptp_step with "H") as (e1' t1'') "[% H]"; first by eauto; simplify_eq.
-  subst. iModIntro; iNext; iMod "H" as ">H". by iApply IH.
-Qed.
-
-Lemma bupd_iter_laterN_mono n P Q `{!Plain Q} :
-  (P ⊢ Q) → Nat.iter n (λ P, |==> ▷ P)%I P ⊢ ▷^n Q.
-Proof.
-  intros HPQ. induction n as [|n IH]=> //=. by rewrite IH bupd_plain.
-Qed.
-
-Lemma bupd_iter_frame_l n R Q :
-  R ∗ Nat.iter n (λ P, |==> ▷ P) Q ⊢ Nat.iter n (λ P, |==> ▷ P) (R ∗ Q).
-Proof.
-  induction n as [|n IH]; simpl; [done|].
-  by rewrite bupd_frame_l {1}(later_intro R) -later_sep IH.
+  iMod (wptp_step with "H") as (e1' t1'') "[% H]"; first eauto; simplify_eq.
+  iMod "H". iModIntro; iNext. iMod "H". iModIntro.
+  by iApply IH.
 Qed.
 
 Lemma wptp_result s n e1 t1 κs κs' v2 t2 σ1 σ2 φ :
   nsteps n (e1 :: t1, σ1) κs (of_val v2 :: t2, σ2) →
-  world σ1 (κs ++ κs') ∗
+  state_interp σ1 (κs ++ κs') ∗
   WP e1 @ s; ⊤ {{ v, ∀ σ, state_interp σ κs' ={⊤,∅}=∗ ⌜φ v σ⌝ }} ∗
-  wptp s t1
-  ⊢ ▷^(S (S n)) ⌜φ v2 σ2⌝.
+  wptp s t1 ⊢
+  |={⊤, ∅}▷=>^(S n) ⌜φ v2 σ2⌝.
 Proof.
-  intros. rewrite wptp_steps // laterN_later. apply: bupd_iter_laterN_mono.
-  iDestruct 1 as (e2 t2' ?) "((Hw & HE & Hσ) & H & _)"; simplify_eq.
-  iDestruct (wp_value_inv' with "H") as "H". rewrite uPred_fupd_eq.
-  iMod ("H" with "[$]") as ">(Hw & HE & H)".
-  iMod ("H" with "Hσ [$]") as ">(_ & _ & $)".
+  intros. rewrite Nat_iter_S_r wptp_steps //.
+  apply step_fupdN_mono.
+  iDestruct 1 as (e2 t2' ?) "(Hσ & H & _)"; simplify_eq.
+  iMod (wp_value_inv' with "H") as "H".
+  iMod (later_fupd_plain false ⊤ ∅ (⌜φ v2 σ2⌝)%I with "[H Hσ]") as ">#%".
+  { rewrite //=. by iMod ("H" with "Hσ") as "$". }
+  iApply (step_fupd_mask_mono ∅ _ _ ∅); auto.
 Qed.
 
 Lemma wp_safe E e σ κs Φ :
-  world' E σ κs -∗ WP e @ E {{ Φ }} ==∗ ▷ ⌜is_Some (to_val e) ∨ reducible e σ⌝.
+  state_interp σ κs -∗ WP e @ E {{ Φ }} ={E, ∅}▷=∗ ⌜is_Some (to_val e) ∨ reducible e σ⌝.
 Proof.
-  rewrite wp_unfold /wp_pre. iIntros "(Hw&HE&Hσ) H".
+  rewrite wp_unfold /wp_pre. iIntros "Hσ H".
   destruct (to_val e) as [v|] eqn:?.
-  { iIntros "!> !> !%". left. by exists v. }
-  rewrite uPred_fupd_eq. iMod ("H" $! _ [] with "Hσ [-]") as ">(?&?&%&?)"; first by iFrame.
-  iIntros "!> !> !%". by right.
+  { iApply (step_fupd_mask_mono ∅ _ _ ∅); eauto. set_solver. }
+  iMod (later_fupd_plain false E ∅ (⌜reducible e σ⌝)%I with "[H Hσ]") as ">#%".
+  { rewrite //=. by iMod ("H" $! σ [] κs with "Hσ") as "($&H)". }
+  iApply step_fupd_intro; first by set_solver+. 
+  iIntros "!> !%". by right.
 Qed.
 
 Lemma wptp_safe n e1 κs κs' e2 t1 t2 σ1 σ2 Φ :
   nsteps n (e1 :: t1, σ1) κs (t2, σ2) → e2 ∈ t2 →
-  world σ1 (κs ++ κs') ∗ WP e1 {{ Φ }} ∗ wptp NotStuck t1
-  ⊢ ▷^(S (S n)) ⌜is_Some (to_val e2) ∨ reducible e2 σ2⌝.
+  state_interp σ1 (κs ++ κs') ∗ WP e1 {{ Φ }} ∗ wptp NotStuck t1
+  ⊢ |={⊤, ∅}▷=>^(S n) ⌜is_Some (to_val e2) ∨ reducible e2 σ2⌝.
 Proof.
-  intros ? He2. rewrite wptp_steps // laterN_later. apply: bupd_iter_laterN_mono.
+  intros ? He2. rewrite Nat_iter_S_r wptp_steps //.
+  apply step_fupdN_mono.
   iDestruct 1 as (e2' t2' ?) "(Hw & H & Htp)"; simplify_eq.
   apply elem_of_cons in He2 as [<-|?].
-  - iMod (wp_safe with "Hw H") as "$".
-  - iMod (wp_safe with "Hw [Htp]") as "$". by iApply (big_sepL_elem_of with "Htp").
+  - iMod (wp_safe with "Hw H") as "$"; auto.
+  - iMod (wp_safe with "Hw [Htp]") as "$"; auto. by iApply (big_sepL_elem_of with "Htp").
 Qed.
 
 Lemma wptp_invariance s n e1 κs κs' e2 t1 t2 σ1 σ2 φ Φ :
   nsteps n (e1 :: t1, σ1) κs (t2, σ2) →
-  (state_interp σ2 κs' ={⊤,∅}=∗ ⌜φ⌝) ∗ world σ1 (κs ++ κs') ∗ WP e1 @ s; ⊤ {{ Φ }} ∗ wptp s t1
-  ⊢ ▷^(S (S n)) ⌜φ⌝.
+  (state_interp σ2 κs' ={⊤,∅}=∗ ⌜φ⌝) ∗ state_interp σ1 (κs ++ κs') ∗ WP e1 @ s; ⊤ {{ Φ }} ∗ wptp s t1
+  ⊢ |={⊤, ∅}▷=>^(S n) |={⊤,∅}=> ⌜φ⌝.
 Proof.
-  intros ?. rewrite wptp_steps // bupd_iter_frame_l laterN_later.
-  apply: bupd_iter_laterN_mono.
-  iIntros "[Hback H]"; iDestruct "H" as (e2' t2' ->) "[(Hw&HE&Hσ) _]".
-  rewrite uPred_fupd_eq.
-  iMod ("Hback" with "Hσ [$Hw $HE]") as "> (_ & _ & $)"; auto.
+  intros ?. rewrite Nat_iter_S_r wptp_steps // step_fupdN_frame_l.
+  apply step_fupdN_mono.
+  iIntros "[Hback H]"; iDestruct "H" as (e2' t2' ->) "[Hσ _]".
+  iSpecialize ("Hback" with "Hσ").
+  iApply (step_fupd_mask_mono ∅ _ _ ∅); auto.
 Qed.
 End adequacy.
 
@@ -183,17 +146,18 @@ Theorem wp_strong_adequacy Σ Λ `{invPreG Σ} s e σ φ :
 Proof.
   intros Hwp; split.
   - intros t2 σ2 v2 [n [κs ?]]%erased_steps_nsteps.
-    eapply (soundness (M:=iResUR Σ) _ (S (S n))).
-    iMod wsat_alloc as (Hinv) "[Hw HE]". specialize (Hwp _ κs).
-    rewrite {1}uPred_fupd_eq in Hwp; iMod (Hwp with "[$Hw $HE]") as ">(Hw & HE & Hwp)".
-    iDestruct "Hwp" as (Istate) "[HI Hwp]".
-    iApply (@wptp_result _ _ (IrisG _ _ _ Hinv Istate) _ _ _ _ _ []); first by eauto.
-    rewrite app_nil_r. eauto with iFrame.
+    eapply (step_fupdN_soundness' _ (S (S n))).
+    iIntros (Hinv).
+    rewrite Nat_iter_S.
+    iMod Hwp as (Istate) "[HI Hwp]".
+    iApply (step_fupd_mask_mono ∅ _ _ ∅); auto. iModIntro. iNext; iModIntro.
+    iApply (@wptp_result _ _ (IrisG _ _ _ Hinv Istate) _ _ _ _ _ []); eauto with iFrame.
   - destruct s; last done. intros t2 σ2 e2 _ [n [κs ?]]%erased_steps_nsteps ?.
-    eapply (soundness (M:=iResUR Σ) _ (S (S n))).
-    iMod wsat_alloc as (Hinv) "[Hw HE]". specialize (Hwp _ κs).
-    rewrite uPred_fupd_eq in Hwp; iMod (Hwp with "[$Hw $HE]") as ">(Hw & HE & Hwp)".
-    iDestruct "Hwp" as (Istate) "[HI Hwp]".
+    eapply (step_fupdN_soundness' _ (S (S n))).
+    iIntros (Hinv).
+    rewrite Nat_iter_S.
+    iMod Hwp as (Istate) "[HI Hwp]".
+    iApply (step_fupd_mask_mono ∅ _ _ ∅); auto.
     iApply (@wptp_safe _ _ (IrisG _ _ _ Hinv Istate) _ _ _ []); [by eauto..|].
     rewrite app_nil_r. eauto with iFrame.
 Qed.
@@ -220,10 +184,11 @@ Theorem wp_invariance Σ Λ `{invPreG Σ} s e σ1 t2 σ2 φ :
   φ.
 Proof.
   intros Hwp [n [κs ?]]%erased_steps_nsteps.
-  eapply (soundness (M:=iResUR Σ) _ (S (S n))).
-  iMod wsat_alloc as (Hinv) "[Hw HE]". specialize (Hwp _ κs []).
-  rewrite {1}uPred_fupd_eq in Hwp; iMod (Hwp with "[$Hw $HE]") as ">(Hw & HE & Hwp)".
-  iDestruct "Hwp" as (Istate) "(HIstate & Hwp & Hclose)".
+  eapply (step_fupdN_soundness _ (S (S n))).
+  iIntros (Hinv).
+  rewrite Nat_iter_S.
+  iMod (Hwp Hinv κs []) as (Istate) "(HIstate & Hwp & Hclose)".
+  iApply (step_fupd_mask_mono ∅ _ _ ∅); auto.
   iApply (@wptp_invariance _ _ (IrisG _ _ _ Hinv Istate)); eauto with iFrame.
 Qed.
 
